theories/language/metatheory.v
@@ -1,7 +1,3 @@
-From stdpp Require Import
-  gmap
-  stringmap.
-
 From zebre Require Import
   prelude.
 From zebre.language Require Export
@@ -9,127 +5,80 @@ From zebre.language Require Export
 From zebre Require Import
   options.
 
-#[local] Definition set_binder_insert x X : stringset :=
-  match x with
-  | BAnon =>
-      X
-  | BNamed f =>
-      {[f]} ∪ X
-  end.
-
-Fixpoint expr_closed X e :=
+Fixpoint occurs x e :=
   match e with
-  | Val v =>
-      val_closed v
-  | Var x =>
-      bool_decide (x ∈ X)
-  | Rec f x e =>
-      expr_closed (set_binder_insert f (set_binder_insert x X)) e
-  | Unop _ e
-  | Proj _ e
-  | Fork e
-  | Load e =>
-      expr_closed X e
-  | App e1 e2
-  | Binop _ e1 e2
-  | Equal e1 e2
-  | Alloc e1 e2
-  | Store e1 e2
-  | Xchg e1 e2
-  | Faa e1 e2 =>
-      expr_closed X e1 && expr_closed X e2
-  | If e0 e1 e2
-  | Cas e0 e1 e2
-  | Resolve e0 e1 e2 =>
-      expr_closed X e0 && expr_closed X e1 && expr_closed X e2
-  | Tuple es
-  | Constr _ es
+  | Val _ =>
+      false
+  | Var y =>
+      bool_decide (x = y)
+  | Rec f y e =>
+      bool_decide (BNamed x ≠ f) &&
+      bool_decide (BNamed x ≠ y) &&
+      occurs x e
+  | App e1 e2 =>
+      occurs x e1 ||
+      occurs x e2
+  | Unop _ e =>
+      occurs x e
+  | Binop _ e1 e2 =>
+      occurs x e1 ||
+      occurs x e2
+  | Equal e1 e2 =>
+      occurs x e1 ||
+      occurs x e2
+  | If e0 e1 e2 =>
+      occurs x e0 ||
+      occurs x e1 ||
+      occurs x e2
+  | Tuple es =>
+      existsb (occurs x) es
+  | Proj _ e =>
+      occurs x e
+  | Constr _ es =>
+      existsb (occurs x) es
+  | Case e0 y e1 brs =>
+      occurs x e0 ||
+      bool_decide (BNamed x ≠ y) && occurs x e1 ||
+      existsb (λ br,
+        let pat := br.1 in
+        forallb (λ y, bool_decide (BNamed x ≠ y)) pat.(pattern_fields) &&
+        bool_decide (BNamed x ≠ pat.(pattern_as)) &&
+        occurs x br.2
+      ) brs
+  | Fork e =>
+      occurs x e
   | Record es =>
-      forallb (expr_closed X) es
-  | Case e0 e1 brs =>
-      expr_closed X e0 && expr_closed X e1 && forallb (λ br, expr_closed X br.2) brs
+      existsb (occurs x) es
+  | Alloc e1 e2 =>
+      occurs x e1 ||
+      occurs x e2
+  | Load e =>
+      occurs x e
+  | Store l e =>
+      occurs x l ||
+      occurs x e
+  | Xchg e1 e2 =>
+      occurs x e1 ||
+      occurs x e2
+  | Cas e0 e1 e2 =>
+      occurs x e0 ||
+      occurs x e1 ||
+      occurs x e2
+  | Faa e1 e2 =>
+      occurs x e1 ||
+      occurs x e2
   | Proph =>
-      true
-  end
-with val_closed v :=
-  match v with
-  | ValLiteral _ =>
-      true
-  | ValRec f x e =>
-      expr_closed (set_binder_insert f (set_binder_insert x ∅)) e
-  | ValTuple vs =>
-      forallb val_closed vs
-  | ValConstr _ vs =>
-      forallb val_closed vs
+      false
+  | Resolve e0 e1 e2 =>
+      occurs x e0 ||
+      occurs x e1 ||
+      occurs x e2
   end.
 
-#[local] Instance set_unfold_elem_of_insert_binder x y X Q :
-  SetUnfoldElemOf y X Q →
-  SetUnfoldElemOf y (set_binder_insert x X) (Q ∨ BNamed y = x).
-Proof.
-  destruct 1; constructor; destruct x; set_solver.
-Qed.
-
-Lemma subst_closed X e x v :
-  expr_closed X e →
-  x ∉ X →
-  subst x v e = e.
-Proof.
-  move: X. induction e => X /=;
-    rewrite ?bool_decide_spec ?andb_True => ? ?;
-    repeat case_decide; simplify_eq/=; f_equal; intuition eauto with set_solver.
-  all: select (Forall _ _) ltac:(fun H => induction H; first done).
-  all: try select branch ltac:(fun br => destruct br).
-  all: rewrite fmap_cons; repeat f_equal; naive_solver.
-Qed.
-
-Lemma subst_closed_empty e x v :
-  expr_closed ∅ e →
-  subst x v e = e.
-Proof.
-  intros. apply subst_closed with (∅ : stringset); set_solver.
-Qed.
-
-Lemma subst_subst e x v v' :
-  subst x v (subst x v' e) = subst x v' e.
-Proof.
-  intros. induction e; simpl; try (f_equal; auto; done);
-    simplify_option_eq; auto using subst_closed_empty with f_equal.
-  all: select (Forall _ _) ltac:(fun H => induction H).
-  all: naive_solver congruence.
-Qed.
-Lemma subst_subst' e x v v' :
-  subst' x v (subst' x v' e) = subst' x v' e.
-Proof.
-  destruct x; simpl; auto using subst_subst.
-Qed.
-
-Lemma subst_subst_ne e x y v v' :
-  x ≠ y →
-  subst x v (subst y v' e) = subst y v' (subst x v e).
-Proof.
-  intros. induction e; simpl; try (f_equal; by auto);
-    simplify_option_eq; auto using eq_sym, subst_closed_empty with f_equal.
-  all: select (Forall _ _) ltac:(fun H => induction H).
-  all: naive_solver congruence.
-Qed.
-Lemma subst_subst_ne' e x y v v' :
-  x ≠ y →
-  subst' x v (subst' y v' e) = subst' y v' (subst' x v e).
-Proof.
-  destruct x, y; simpl; auto using subst_subst_ne with congruence.
-Qed.
-
-Lemma subst_rec' f y e x v :
-  x = f ∨ x = y ∨ x = BAnon →
-  subst' x v (Rec f y e) = Rec f y e.
-Proof.
-  intros. destruct x; simplify_option_eq; naive_solver.
-Qed.
-Lemma subst_rec_ne' f y e x v :
-  (x ≠ f ∨ f = BAnon) →
-  (x ≠ y ∨ y = BAnon) →
-  subst' x v (Rec f y e) = Rec f y (subst' x v e).
-Proof.
-  intros. destruct x; simplify_option_eq; naive_solver.
-Qed.
+Definition val_recursive v :=
+  match v with
+  | ValRec (BNamed f) x e =>
+      occurs f e
+  | _ =>
+      false
+  end.
